Make a cv-translated version of the semantics

vyperVmScript.sml
@@ -1,8 +1,136 @@
-open HolKernel boolLib bossLib Parse
-open listTheory alistTheory finite_mapTheory
+open HolKernel boolLib bossLib Parse dep_rewrite
+open listTheory alistTheory finite_mapTheory arithmeticTheory
+     numposrepTheory stringTheory combinTheory
+     cv_typeTheory cv_stdTheory cv_transLib
 open vyperAstTheory vfmContextTheory
 
 val () = new_theory "vyperVm";
+
+Definition string_to_num_def:
+  string_to_num s = l2n 257 (MAP (SUC o ORD) s)
+End
+
+Definition MAP_CHR_o_PRE_def:
+  MAP_CHR_o_PRE [] acc = REVERSE acc ∧
+  MAP_CHR_o_PRE (x::xs) acc =
+  MAP_CHR_o_PRE xs (CHR(PRE x)::acc)
+End
+
+val MAP_CHR_o_PRE_pre_def = cv_auto_trans_pre MAP_CHR_o_PRE_def;
+
+Theorem MAP_CHR_o_PRE_pre:
+  EVERY ($> 257) v ==>
+  MAP_CHR_o_PRE_pre v acc
+Proof
+  qid_spec_tac`acc` \\ Induct_on`v`
+  \\ rw[Once MAP_CHR_o_PRE_pre_def]
+QED
+
+Theorem MAP_CHR_o_PRE:
+  MAP_CHR_o_PRE ls acc = REVERSE acc ++ (MAP (CHR o PRE) ls)
+Proof
+  qid_spec_tac`acc` \\ Induct_on`ls`
+  \\ rw[MAP_CHR_o_PRE_def]
+QED
+
+Definition num_to_string_def:
+  num_to_string n =
+  if n = 0 then "" else
+  MAP (CHR o PRE) (n2l 257 n)
+End
+
+Theorem string_to_num_to_string:
+  num_to_string (string_to_num s) = s
+Proof
+  simp[num_to_string_def, string_to_num_def, l2n_eq_0]
+  \\ rw[EVERY_MAP]
+  >- (
+    qmatch_assum_abbrev_tac`EVERY P s`
+    \\ `P = K F`
+    by (
+      rw[Abbr`P`, FUN_EQ_THM]
+      \\ DEP_REWRITE_TAC[LESS_MOD]
+      \\ rw[SUC_LT]
+      \\ qexists_tac`256`
+      \\ simp[ORD_BOUND] )
+    \\ Cases_on`s` \\ gvs[] )
+  \\ DEP_REWRITE_TAC[n2l_l2n]
+  \\ simp[l2n_eq_0, EVERY_MAP]
+  \\ DEP_REWRITE_TAC[LOG_l2n]
+  \\ simp[EVERY_MAP, GREATER_DEF, MAP_TAKE, MAP_MAP_o, o_DEF]
+  \\ Cases_on`s = []` \\ gvs[]
+  \\ rw[SUC_LT, EVERY_MEM]
+  \\ qexists_tac`256`
+  \\ simp[ORD_BOUND]
+QED
+
+val () = cv_auto_trans string_to_num_def;
+
+val num_to_string_pre_def = cv_auto_trans_pre (
+  num_to_string_def
+ |> REWRITE_RULE[
+      MAP_CHR_o_PRE |> Q.GEN`acc` |> Q.SPEC`[]`
+      |> SIMP_RULE std_ss [APPEND, REVERSE_DEF] |> SYM
+    ] )
+
+Theorem num_to_string_pre[cv_pre]:
+  num_to_string_pre n
+Proof
+  rw[num_to_string_pre_def]
+  \\ irule MAP_CHR_o_PRE_pre
+  \\ irule n2l_BOUND
+  \\ rw[]
+QED
+
+(*
+Theorem num_to_string_inj:
+  (* this is false because of 0 digits *)
+  num_to_string x = num_to_string y ==> x = y
+Proof
+  simp[num_to_string_def]
+  \\ qmatch_goalsub_abbrev_tac`n2l b`
+  \\ pop_assum mp_tac
+  \\ simp[markerTheory.Abbrev_def]
+  \\ qid_spec_tac`y`
+  \\ qid_spec_tac`x`
+  \\ qid_spec_tac`b`
+  \\ ho_match_mp_tac n2l_ind
+  \\ rpt gen_tac \\ strip_tac
+  \\ rpt gen_tac \\ strip_tac
+  \\ gvs[]
+  \\ rw[]
+  >- rw[Once n2l_def]
+  >- rw[Once n2l_def]
+  \\ pop_assum mp_tac
+  \\ rw[Once n2l_def]
+  >- (
+    Cases_on`x` \\ gvs[]
+    \\ qpat_x_assum`n2l _ _ = _`mp_tac
+    \\ rw[Once n2l_def]
+    >- ( Cases_on`x0` \\ gvs[] )
+    \\ rw[Once n2l_def] )
+  \\ pop_assum mp_tac
+  \\ simp[Once n2l_def, SimpRHS]
+  \\ rw[]
+  >- rw[Once n2l_def]
+  \\ gs[]
+  \\ qspec_then`257`mp_tac DIVISION
+  \\ impl_tac >- rw[]
+  \\ disch_then(fn th => qspec_then`x`mp_tac th \\ qspec_then`y`mp_tac th)
+  \\ ntac 2 strip_tac
+  \\ qpat_x_assum`x = _`SUBST1_TAC
+  \\ qpat_x_assum`y = _`SUBST1_TAC
+  \\ qmatch_goalsub_abbrev_tac`xd * _ + xm = yd * _ + ym`
+  \\ `xd = yd ∧ xm = ym` suffices_by rw[]
+  \\ `PRE xm < 256` by (Cases_on`xm` \\ gvs[])
+  \\ `PRE ym < 256` by (Cases_on`ym` \\ gvs[])
+  \\ gs[]
+  \\ Cases_on`xm = 0` >- (
+    gvs[Abbr`xm`, MOD_EQ_0_IFF]
+
+  m``PRE 0``
+
+*)
 
 Datatype:
   value
@@ -23,17 +151,63 @@ End
 Definition default_value_def:
   default_value (BaseT (UintT _)) = IntV 0 ∧
   default_value (BaseT (IntT _)) = IntV 0 ∧
-  default_value (TupleT ts) = TupleV (MAP default_value ts) ∧
+  default_value (TupleT ts) = TupleV (default_value_list ts) ∧
   default_value (DynArrayT _ _) = ArrayV [] ∧
   default_value VoidT = VoidV ∧
   default_value (BaseT BoolT) = BoolV F ∧
   default_value (BaseT StringT) = StringV "" ∧
-  default_value (BaseT BytesT) = BytesV []
+  default_value (BaseT BytesT) = BytesV [] ∧
+  default_value_list [] = [] ∧
+  default_value_list (t::ts) = default_value t :: default_value_list ts
 Termination
-  WF_REL_TAC ‘measure type_size’
+  WF_REL_TAC ‘measure
+    (λx. case x of INR t => type1_size t | INL t => type_size t)’
 End
 
+Theorem default_value_list_MAP:
+  default_value_list ls = MAP default_value ls
+Proof
+  Induct_on`ls` \\ rw[default_value_def]
+QED
+
+val () = cv_auto_trans default_value_def;
+
+(*
+We don't use this directly to support cv which prefers num keys
 Type scope = “:identifier |-> value”;
+*)
+Type scope = “:num |-> value”;
+
+val from_to_value_thm = cv_typeLib.from_to_thm_for “:value”;
+val from_value = from_to_value_thm |> concl |> rator |> rand
+val to_value = from_to_value_thm |> concl |> rand
+
+(*
+Definition from_scope_def:
+  from_scope env = from_fmap ^from_value (env f_o num_to_string)
+End
+
+Definition to_scope_def:
+  to_scope cv = to_fmap ^to_value cv f_o string_to_num
+End
+
+Theorem from_to_scope[cv_from_to]:
+  from_to from_scope to_scope
+Proof
+  mp_tac $ MATCH_MP from_to_fmap from_to_value_thm
+  \\ rw[from_to_def, from_scope_def, to_scope_def]
+  \\ DEP_REWRITE_TAC[f_o_ASSOC]
+  \\ rw[EQ_IMP_THM]
+  >- cheat
+  >- metis_tac[string_to_num_to_string]
+  \\ irule (iffLR fmap_EQ_THM)
+  \\ DEP_REWRITE_TAC[FDOM_f_o]
+  \\ simp[o_DEF, string_to_num_to_string]
+  \\ rw[]
+  \\ DEP_REWRITE_TAC[FAPPLY_f_o]
+  \\ simp[]
+QED
+*)
 
 Definition lookup_scopes_def:
   lookup_scopes id [] = NONE ∧
@@ -42,6 +216,11 @@ Definition lookup_scopes_def:
     lookup_scopes id rest
   | SOME v => SOME v
 End
+
+(*
+TODO: somehow rework to use num_maps?
+val () = cv_auto_trans lookup_scopes_def;
+*)
 
 Datatype:
   expr_continuation
@@ -137,6 +316,8 @@ Definition evaluate_literal_def:
   evaluate_literal (IntL i)    = IntV i
 End
 
+val () = cv_auto_trans evaluate_literal_def;
+
 Definition evaluate_cmp_def:
   evaluate_cmp Eq    (StringV s1) (StringV s2) = DoneExpr (BoolV (s1 = s2)) ∧
   evaluate_cmp Eq    (IntV i1)    (IntV i2)    = DoneExpr (BoolV (i1 = i2)) ∧
@@ -145,11 +326,15 @@ Definition evaluate_cmp_def:
   evaluate_cmp _ _ _ = ErrorExpr
 End
 
+val () = cv_auto_trans evaluate_cmp_def;
+
 Definition evaluate_binop_def:
   evaluate_binop Add (IntV i1) (IntV i2) = DoneExpr (IntV (i1 + i2)) ∧
   evaluate_binop Sub (IntV i1) (IntV i2) = DoneExpr (IntV (i1 - i2)) ∧
   evaluate_binop (_: operator) _ _ = ErrorExpr
 End
+
+val () = cv_auto_trans evaluate_binop_def;
 
 Definition extract_elements_def:
   extract_elements (ArrayV vs) = SOME vs ∧
@@ -157,11 +342,15 @@ Definition extract_elements_def:
   extract_elements _ = NONE
 End
 
+val () = cv_auto_trans extract_elements_def;
+
 Definition replace_elements_def:
   replace_elements (ArrayV _) vs = SOME (ArrayV vs) ∧
   replace_elements (TupleV _) vs = SOME (TupleV vs) ∧
   replace_elements _ _ = NONE
 End
+
+val () = cv_auto_trans replace_elements_def;
 
 Definition integer_index_def:
   integer_index vs i =
@@ -169,6 +358,8 @@ Definition integer_index_def:
      SOME $ if 0 ≤ i then Num i else LENGTH vs - Num i
    else NONE
 End
+
+val () = cv_auto_trans integer_index_def;
 
 Definition evaluate_subscript_def:
   evaluate_subscript av (IntV i) =
@@ -179,12 +370,25 @@ Definition evaluate_subscript_def:
   evaluate_subscript _ _ = ErrorExpr
 End
 
+val evaluate_subscript_pre_def = cv_auto_trans_pre evaluate_subscript_def;
+
+Theorem evaluate_subscript_pre[cv_pre]:
+  evaluate_subscript_pre av v
+Proof
+  rw[evaluate_subscript_pre_def, integer_index_def]
+  \\ rw[]
+  \\ qmatch_asmsub_rename_tac`0i ≤ v0`
+  \\ Cases_on`v0` \\ gs[]
+QED
+
 Definition evaluate_attribute_def:
   evaluate_attribute (StructV kvs) id =
   (case ALOOKUP kvs id of SOME v => DoneExpr v
    | _ => ErrorExpr) ∧
   evaluate_attribute _ _ = ErrorExpr
 End
+
+val () = cv_auto_trans evaluate_attribute_def;
 
 Definition step_expr_def:
   step_expr gbs env (StartExpr (Literal l)) =
@@ -194,11 +398,11 @@ Definition step_expr_def:
   step_expr gbs env (StartExpr (ArrayLit (e::es))) =
     ArrayLitK [] (StartExpr e) es ∧
   step_expr gbs env (StartExpr (Name id)) =
-    (case lookup_scopes id env
+    (case lookup_scopes (string_to_num id) env
      of SOME v => DoneExpr v
       | _ => ErrorExpr) ∧
   step_expr gbs env (StartExpr (GlobalName id)) =
-    (case FLOOKUP gbs id
+    (case FLOOKUP gbs (string_to_num id)
      of SOME (Value v) => DoneExpr v
       | _ => ErrorExpr) ∧
   step_expr gbs env (StartExpr (Subscript e1 e2)) =
@@ -298,9 +502,11 @@ Definition step_expr_def:
   step_expr gbs env ErrorExpr = ErrorExpr
 End
 
+val () = cv_auto_trans step_expr_def;
+
 Datatype:
   loop_info = <|
-    loop_var: identifier
+    loop_var: (* identifier *) num
   ; loop_first_stmt: stmt
   ; loop_rest_stmts: stmt list
   ; remaining_values: value list
@@ -320,7 +526,7 @@ Datatype:
   execution_context = <|
     current_fc : function_context
   ; call_stack : function_context list
-  ; globals: identifier |-> toplevel_value
+  ; globals: (* identifier *) num |-> toplevel_value
   ; contract: toplevel list
   |>
 End
@@ -334,17 +540,21 @@ Definition initial_function_context_def:
   |>
 End
 
+val () = cv_auto_trans initial_function_context_def;
+
 (* TODO: assumes unique identifiers, but should check? *)
 Definition initial_globals_def:
   initial_globals [] = FEMPTY ∧
   initial_globals (VariableDecl id typ _ Storage :: ts) =
-  initial_globals ts |+ (id, Value $ default_value typ) ∧
+  initial_globals ts |+ (string_to_num id, Value $ default_value typ) ∧
   initial_globals (VariableDecl id typ _ Transient :: ts) =
-  initial_globals ts |+ (id, Value $ default_value typ) ∧
+  initial_globals ts |+ (string_to_num id, Value $ default_value typ) ∧
   (* TODO: handle Constants and  Immutables *)
   initial_globals (t :: ts) = initial_globals ts
   (* TODO: hashmap toplevels *)
 End
+
+val () = cv_auto_trans initial_globals_def;
 
 Definition initial_execution_context_def:
   initial_execution_context ts fc = <|
@@ -355,15 +565,21 @@ Definition initial_execution_context_def:
   |>
 End
 
+val () = cv_auto_trans initial_execution_context_def;
+
 Definition raise_def:
   raise err ctx = ctx with current_fc updated_by
     (λfc. fc with current_stmt := ExceptionK err)
 End
 
+val () = cv_auto_trans raise_def;
+
 Definition push_scope_def:
   push_scope ctx =
     ctx with current_fc updated_by (λfc. fc with scopes updated_by CONS FEMPTY)
 End
+
+val () = cv_auto_trans push_scope_def;
 
 Definition pop_scope_def:
   pop_scope ctx =
@@ -371,6 +587,8 @@ Definition pop_scope_def:
     of [] => raise Error ctx
      | (_::rest) => ctx with current_fc updated_by (λfc. fc with scopes := rest)
 End
+
+val () = cv_auto_trans pop_scope_def;
 
 Definition new_variable_def:
   new_variable id typ ctx =
@@ -382,6 +600,8 @@ Definition new_variable_def:
            (λfc. fc with scopes := (env |+ (id, default_value typ))::rest)
 End
 
+val () = cv_auto_trans (REWRITE_RULE[TO_FLOOKUP]new_variable_def);
+
 Definition find_containing_scope_def:
   find_containing_scope id [] = NONE : containing_scope option ∧
   find_containing_scope id (env::rest) =
@@ -389,9 +609,11 @@ Definition find_containing_scope_def:
   else OPTION_MAP (λ(p,q). (env::p, q)) (find_containing_scope id rest)
 End
 
+val () = cv_auto_trans (REWRITE_RULE[TO_FLOOKUP]find_containing_scope_def);
+
 Definition step_base_target_def:
   step_base_target gbs env (StartBaseTgt (NameTarget id)) =
-    (case find_containing_scope id env
+    (case find_containing_scope (string_to_num id) env
      of SOME cs => SOME $ DoneBaseTgt (ScopedVar cs id) []
       | _ => NONE) ∧
   step_base_target gbs env (StartBaseTgt (GlobalNameTarget id)) =
@@ -423,8 +645,14 @@ Definition step_base_target_def:
     | SOME (LiftCallBaseTgt fn vs k) =>
         SOME $ LiftCallBaseTgt fn vs (AttributeTargetK k id)
     | SOME k => SOME $ AttributeTargetK k id
-    | _ => NONE)
+    | _ => NONE) ∧
+  step_base_target gbs env (LiftCallBaseTgt fn vs k) =
+    SOME $ LiftCallBaseTgt fn vs k ∧
+  step_base_target gbs env (DoneBaseTgt l s) =
+    SOME $ DoneBaseTgt l s
 End
+
+val () = cv_auto_trans step_base_target_def;
 
 Definition step_target_def:
   step_target gbs env (StartTgt (BaseTarget b)) =
@@ -453,6 +681,8 @@ Definition step_target_def:
   step_target gbs env _ = ErrorTgt
 End
 
+val () = cv_auto_trans step_target_def;
+
 Definition set_variable_def:
   set_variable id v ctx =
   case find_containing_scope id ctx.current_fc.scopes
@@ -462,6 +692,8 @@ Definition set_variable_def:
          ctx with current_fc updated_by
            (λfc. fc with scopes := pre ++ (env |+ (id, v))::rest)
 End
+
+val () = cv_auto_trans set_variable_def;
 
 Definition assign_subscripts_def:
   assign_subscripts a [] v = SOME v ∧
@@ -476,31 +708,50 @@ Definition assign_subscripts_def:
   assign_subscripts a _ v = NONE (* TODO: handle AttrSubscript *)
 End
 
+val assign_subscripts_pre_def = cv_auto_trans_pre assign_subscripts_def;
+
+Theorem assign_subscripts_pre[cv_pre]:
+  !a b c. assign_subscripts_pre a b c
+Proof
+  ho_match_mp_tac assign_subscripts_ind
+  \\ rw[Once assign_subscripts_pre_def]
+  \\ rw[Once assign_subscripts_pre_def]
+  \\ gvs[integer_index_def] \\ rw[]
+  \\ qmatch_asmsub_rename_tac`0i ≤ v0`
+  \\ Cases_on`v0` \\ gs[]
+QED
+
 Definition assign_target_def:
   assign_target (BaseTargetV (ScopedVar (pre,env,rest) id) is) v ctx =
-    (case FLOOKUP env id of SOME a =>
+    (let nid = string_to_num id in
+    (case FLOOKUP env nid of SOME a =>
      (case assign_subscripts a is v of SOME a' =>
         ctx with current_fc updated_by
-          (λfc. fc with scopes := pre ++ (env |+ (id, a'))::rest)
+          (λfc. fc with scopes := pre ++ (env |+ (nid, a'))::rest)
       | _ => raise Error ctx)
-     | _ => raise Error ctx) ∧
+     | _ => raise Error ctx)) ∧
   assign_target (BaseTargetV (Global id) is) v ctx =
+  (let nid = string_to_num id in
   (* TODO: add assignment to hashmaps *)
-  (case FLOOKUP ctx.globals id of SOME (Value a) =>
+  (case FLOOKUP ctx.globals nid of SOME (Value a) =>
    (case assign_subscripts a is v of SOME a' =>
-     ctx with globals := ctx.globals |+ (id, Value a')
+     ctx with globals := ctx.globals |+ (nid, Value a')
     | _ => raise Error ctx)
-   | _ => raise Error ctx) ∧
+   | _ => raise Error ctx)) ∧
   assign_target _ _ ctx = raise Error ctx (* TODO: handle TupleTargetV *)
 End
+
+val () = cv_auto_trans assign_target_def;
 
 (* TODO: check types? *)
 Definition bind_arguments_def:
   bind_arguments ([]: argument list) [] = SOME (FEMPTY: scope) ∧
   bind_arguments ((id, typ)::params) (v::vs) =
-    OPTION_MAP (λm. m |+ (id, v)) (bind_arguments params vs) ∧
+    OPTION_MAP (λm. m |+ (string_to_num id, v)) (bind_arguments params vs) ∧
   bind_arguments _ _ = NONE
 End
+
+val () = cv_auto_trans bind_arguments_def;
 
 Definition lookup_external_function_def:
   lookup_external_function name [] = NONE ∧
@@ -510,6 +761,8 @@ Definition lookup_external_function_def:
   lookup_external_function name (_ :: ts) =
     lookup_external_function name ts
 End
+
+val () = cv_auto_trans lookup_external_function_def;
 
 Definition push_call_def:
   push_call fn args ctx =
@@ -525,29 +778,35 @@ Definition push_call_def:
   | _ => raise Error ctx
 End
 
+val () = cv_auto_trans push_call_def;
+
 Definition update_current_stmt_def:
   update_current_statement st ctx =
   ctx with current_fc updated_by
     (λfc. fc with current_stmt := st)
 End
 
+val () = cv_auto_trans update_current_stmt_def;
+
 Definition return_expr_def:
   return_expr v (StartExpr _) = ErrorExpr ∧
   return_expr v (IfExpK k e1 e2) = IfExpK (return_expr v k) e1 e2  ∧
   return_expr v (ArrayLitK vs k es) = ArrayLitK vs (return_expr v k) es ∧
   return_expr v (SubscriptK1 k e) = SubscriptK1 (return_expr v k) e ∧
-  return_expr v (SubscriptK2 v k) = SubscriptK2 v (return_expr v k) ∧
+  return_expr v (SubscriptK2 w k) = SubscriptK2 w (return_expr v k) ∧
   return_expr v (AttributeK k id) = AttributeK (return_expr v k) id ∧
   return_expr v (CompareK1 k cmp e) = CompareK1 (return_expr v k) cmp e ∧
-  return_expr v (CompareK2 v cmp k) = CompareK2 v cmp (return_expr v k) ∧
+  return_expr v (CompareK2 w cmp k) = CompareK2 w cmp (return_expr v k) ∧
   return_expr v (BinOpK1 k bop e) = BinOpK1 (return_expr v k) bop e ∧
-  return_expr v (BinOpK2 v bop k) = BinOpK2 v bop (return_expr v k) ∧
+  return_expr v (BinOpK2 w bop k) = BinOpK2 w bop (return_expr v k) ∧
   return_expr v (CallK id vs k es) = CallK id vs (return_expr v k) es ∧
   return_expr v (LiftCall fn vs k) = LiftCall fn vs (return_expr v k) ∧
   return_expr v (DoneExpr _) = ErrorExpr ∧
   return_expr v ReturnExpr = DoneExpr v ∧
   return_expr v ErrorExpr = ErrorExpr
 End
+
+val () = cv_auto_trans return_expr_def;
 
 Definition return_base_tgt_def:
   return_base_tgt v (StartBaseTgt _) = NONE ∧
@@ -562,6 +821,8 @@ Definition return_base_tgt_def:
   return_base_tgt _ _ = NONE
 End
 
+val () = cv_auto_trans return_base_tgt_def;
+
 Definition return_tgt_def:
   return_tgt v (StartTgt _) = ErrorTgt ∧
   return_tgt v (TupleTargetK vs k as) =
@@ -575,6 +836,8 @@ Definition return_tgt_def:
   return_tgt v ErrorTgt = ErrorTgt
 End
 
+val () = cv_auto_trans return_tgt_def;
+
 Definition return_def:
   return v (ForK id typ k ss) = ForK id typ (return_expr v k) ss ∧
   return v (IfK k s1 s2) = IfK (return_expr v k) s1 s2 ∧
@@ -586,6 +849,8 @@ Definition return_def:
   return v (AnnAssignK id typ k) = AnnAssignK id typ (return_expr v k) ∧
   return v _ = ExceptionK Error
 End
+
+val () = cv_auto_trans return_def;
 
 Definition pop_call_def:
   pop_call v ctx =
@@ -602,15 +867,36 @@ Termination
   WF_REL_TAC`measure (λx. LENGTH (SND x).call_stack)` \\ rw[]
 End
 
+val pop_call_pre_def = cv_auto_trans_pre pop_call_def;
+
+Theorem pop_call_pre[cv_pre]:
+  ∀v ctx. pop_call_pre v ctx
+Proof
+  ho_match_mp_tac pop_call_ind
+  \\ rw[]
+  \\ rw[Once pop_call_pre_def]
+  \\ fs[]
+  \\ qmatch_assum_abbrev_tac`pop_call_pre v c1`
+  \\ qmatch_goalsub_abbrev_tac`pop_call_pre v c2`
+  \\ `c1 = c2` suffices_by (rw[] \\ fs[])
+  \\ rw[Abbr`c1`, Abbr`c2`]
+  \\ CASE_TAC
+  \\ rw[ theorem"execution_context_component_equality"]
+QED
+
 Definition set_stmt_def:
   set_stmt k ctx =
     ctx with current_fc updated_by (λfc. fc with current_stmt := k)
 End
 
+val () = cv_auto_trans set_stmt_def;
+
 Definition exception_raised_def:
   exception_raised ctx <=>
   case ctx.current_fc.current_stmt of ExceptionK _ => T | _ => F
 End
+
+val () = cv_auto_trans exception_raised_def;
 
 Definition push_loop_def:
   push_loop id typ (v::vs) (s::ss) ctx =
@@ -632,12 +918,16 @@ Definition push_loop_def:
   push_loop _ _ _ _ ctx = raise Error ctx
 End
 
+val () = cv_auto_trans push_loop_def;
+
 Definition pop_loop_def:
   pop_loop ctx =
   case ctx.call_stack of
      | [] => raise Error ctx
      | fc::fcs => ctx with <| current_fc := fc; call_stack := fcs |>
 End
+
+val () = cv_auto_trans pop_loop_def;
 
 Definition next_iteration_def:
   next_iteration li ctx =
@@ -649,6 +939,8 @@ Definition next_iteration_def:
                  ; loop := SOME (li with remaining_values := vs) |>)
 End
 
+val () = cv_auto_trans next_iteration_def;
+
 Definition continue_loop_def:
   continue_loop ctx =
   case ctx.current_fc.loop of SOME li => (
@@ -658,6 +950,8 @@ Definition continue_loop_def:
   ) | _ => raise Error ctx
 End
 
+val () = cv_auto_trans continue_loop_def;
+
 Definition break_loop_def:
   break_loop ctx =
   case ctx.current_fc.loop of SOME li => (
@@ -666,6 +960,8 @@ Definition break_loop_def:
         pop_loop ctx
   ) | _ => raise Error ctx
 End
+
+val () = cv_auto_trans break_loop_def;
 
 Definition next_stmt_def:
   next_stmt ctx =
@@ -677,6 +973,8 @@ Definition next_stmt_def:
             of NONE => pop_call VoidV ctx
              | SOME li => next_iteration li ctx)
 End
+
+val () = cv_auto_trans next_stmt_def;
 
 Definition step_stmt_def:
   step_stmt ctx =
@@ -755,12 +1053,13 @@ Definition step_stmt_def:
           set_stmt
             (AssignK2 tv (step_expr ctx.globals fc.scopes k)) ctx
       | AugAssignK id bop (DoneExpr v2) =>
-        (case lookup_scopes id fc.scopes
+        (let nid = string_to_num id in
+        (case lookup_scopes nid fc.scopes
            of NONE => raise Error ctx
             | SOME v1 =>
               (case evaluate_binop bop v1 v2
-                 of DoneExpr v => set_stmt DoneK (set_variable id v ctx)
-                  | _ => raise Error ctx))
+                 of DoneExpr v => set_stmt DoneK (set_variable nid v ctx)
+                  | _ => raise Error ctx)))
       | AugAssignK id bop ErrorExpr => raise Error ctx
       | AugAssignK id bop ReturnExpr => raise Error ctx
       | AugAssignK id bop (LiftCall fn vs k) =>
@@ -770,9 +1069,10 @@ Definition step_stmt_def:
           set_stmt
             (AugAssignK id bop (step_expr ctx.globals fc.scopes k)) ctx
       | AnnAssignK id typ (DoneExpr v) => (
-          let ctx = new_variable id typ ctx in
+          let nid = string_to_num id in
+          let ctx = new_variable nid typ ctx in
             if exception_raised ctx then ctx else
-              set_stmt DoneK (set_variable id v ctx))
+              set_stmt DoneK (set_variable nid v ctx))
       | AnnAssignK id typ ErrorExpr => raise Error ctx
       | AnnAssignK id typ ReturnExpr => raise Error ctx
       | AnnAssignK id typ (LiftCall fn vs k) =>
@@ -785,7 +1085,7 @@ Definition step_stmt_def:
       | ForK id typ (DoneExpr (ArrayV [])) (st::ss) =>
           set_stmt DoneK ctx
       | ForK id typ (DoneExpr (ArrayV vs)) ss =>
-          push_loop id typ vs ss ctx
+          push_loop (string_to_num id) typ vs ss ctx
       | ForK id typ (DoneExpr _) _ => raise Error ctx
       | ForK id typ ErrorExpr _ => raise Error ctx
       | ForK id typ ReturnExpr _ => raise Error ctx
@@ -795,6 +1095,8 @@ Definition step_stmt_def:
       | ForK id typ k ss =>
           set_stmt (ForK id typ (step_expr ctx.globals fc.scopes k) ss) ctx)
 End
+
+val () = cv_auto_trans step_stmt_def;
 
 Definition external_call_def:
   external_call n name args ts =
@@ -811,5 +1113,7 @@ Definition external_call_def:
      | _ => NONE)
   | _ => NONE
 End
+
+val () = cv_auto_trans external_call_def;
 
 val () = export_theory();
